Auto/Embedding/LamSystem.lean
@@ -1790,7 +1790,7 @@ def LamTerm.emb : LamTerm := .mkForallEF (.base .bool) (.mkOr
   (.mkEq (.base .bool) (.bvar 0) (.base .falseb)))
 
 def LamWF.emb : LamWF ltv ⟨lctx, LamTerm.emb, .base .prop⟩ :=
-  .mkForallEF (.mkOr (.mkEq (.ofBVar 0) (.ofBase .ofTrueB')) (.mkEq (.ofBVar 0) (.ofBase .ofFalseB')))
+  .mkForallEF (.mkOr (.mkEq (.ofBVar 0) (.ofBase .ofTrueB)) (.mkEq (.ofBVar 0) (.ofBase .ofFalseB)))
 
 theorem LamThmValid.emb : LamThmValid lval [] LamTerm.emb := by
   intro lctx'; rw [pushLCtxs_nil]; exists LamWF.emb; intro lctxTerm
@@ -1803,7 +1803,7 @@ theorem LamThmValid.emb : LamThmValid lval [] LamTerm.emb := by
 def LamTerm.false_ne_true : LamTerm := .mkNot (.mkEq (.base .bool) (.base .falseb) (.base .trueb))
 
 def LamWF.false_ne_true : LamWF ltv ⟨lctx, LamTerm.false_ne_true, .base .prop⟩ :=
-  .mkNot (.mkEq (.ofBase .ofFalseB') (.ofBase .ofTrueB'))
+  .mkNot (.mkEq (.ofBase .ofFalseB) (.ofBase .ofTrueB))
 
 theorem LamThmValid.false_ne_true : LamThmValid lval [] LamTerm.false_ne_true := by
   intro lctx'; rw [pushLCtxs_nil]; exists LamWF.false_ne_true; intro lctxTerm
@@ -1813,7 +1813,7 @@ def LamTerm.not_true_eq_false : LamTerm := .mkEq (.base .bool)
   (.app (.base .bool) (.base .notb) (.base .trueb)) (.base .falseb)
 
 def LamWF.not_true_eq_false : LamWF ltv ⟨lctx, LamTerm.not_true_eq_false, .base .prop⟩ :=
-  .mkEq (.ofApp _ (.ofBase .ofNotB') (.ofBase .ofTrueB')) (.ofBase .ofFalseB')
+  .mkEq (.ofApp _ (.ofBase .ofNotB) (.ofBase .ofTrueB)) (.ofBase .ofFalseB)
 
 theorem LamThmValid.not_true_eq_false : LamThmValid lval [] LamTerm.not_true_eq_false := by
   intro lctx'; rw [pushLCtxs_nil]; exists LamWF.not_true_eq_false; intro _; rfl
@@ -1822,7 +1822,7 @@ def LamTerm.not_false_eq_true : LamTerm := .mkEq (.base .bool)
   (.app (.base .bool) (.base .notb) (.base .falseb)) (.base .trueb)
 
 def LamWF.not_false_eq_true : LamWF ltv ⟨lctx, LamTerm.not_false_eq_true, .base .prop⟩ :=
-  .mkEq (.ofApp _ (.ofBase .ofNotB') (.ofBase .ofFalseB')) (.ofBase .ofTrueB')
+  .mkEq (.ofApp _ (.ofBase .ofNotB) (.ofBase .ofFalseB)) (.ofBase .ofTrueB)
 
 theorem LamThmValid.not_false_eq_true : LamThmValid lval [] LamTerm.not_false_eq_true := by
   intro lctx'; rw [pushLCtxs_nil]; exists LamWF.not_false_eq_true; intro _; rfl
@@ -1831,7 +1831,7 @@ def LamTerm.false_and_eq_false : LamTerm := .mkForallEF (.base .bool) (.mkEq (.b
   (.app (.base .bool) (.app (.base .bool) (.base .andb) (.base .falseb)) (.bvar 0)) (.base .falseb))
 
 def LamWF.false_and_eq_false : LamWF ltv ⟨lctx, LamTerm.false_and_eq_false, .base .prop⟩ :=
-  .mkForallEF (.mkEq (.ofApp _ (.ofApp _ (.ofBase .ofAndB') (.ofBase .ofFalseB')) (.ofBVar 0)) (.ofBase .ofFalseB'))
+  .mkForallEF (.mkEq (.ofApp _ (.ofApp _ (.ofBase .ofAndB) (.ofBase .ofFalseB)) (.ofBVar 0)) (.ofBase .ofFalseB))
 
 theorem LamThmValid.false_and_eq_false : LamThmValid lval [] LamTerm.false_and_eq_false := by
   intro lctx'; rw [pushLCtxs_nil]; exists LamWF.false_and_eq_false; intro _ b; rfl
@@ -1840,7 +1840,7 @@ def LamTerm.true_and_eq_id : LamTerm := .mkForallEF (.base .bool) (.mkEq (.base 
   (.app (.base .bool) (.app (.base .bool) (.base .andb) (.base .trueb)) (.bvar 0)) (.bvar 0))
 
 def LamWF.true_and_eq_id : LamWF ltv ⟨lctx, LamTerm.true_and_eq_id, .base .prop⟩ :=
-  .mkForallEF (.mkEq (.ofApp _ (.ofApp _ (.ofBase .ofAndB') (.ofBase .ofTrueB')) (.ofBVar 0)) (.ofBVar 0))
+  .mkForallEF (.mkEq (.ofApp _ (.ofApp _ (.ofBase .ofAndB) (.ofBase .ofTrueB)) (.ofBVar 0)) (.ofBVar 0))
 
 theorem LamThmValid.true_and_eq_id : LamThmValid lval [] LamTerm.true_and_eq_id := by
   intro lctx'; rw [pushLCtxs_nil]; exists LamWF.true_and_eq_id; intro _ b; rfl
@@ -1849,7 +1849,7 @@ def LamTerm.false_or_eq_id : LamTerm := .mkForallEF (.base .bool) (.mkEq (.base 
   (.app (.base .bool) (.app (.base .bool) (.base .orb) (.base .falseb)) (.bvar 0)) (.bvar 0))
 
 def LamWF.false_or_eq_id : LamWF ltv ⟨lctx, LamTerm.false_or_eq_id, .base .prop⟩ :=
-  .mkForallEF (.mkEq (.ofApp _ (.ofApp _ (.ofBase .ofOrB') (.ofBase .ofFalseB')) (.ofBVar 0)) (.ofBVar 0))
+  .mkForallEF (.mkEq (.ofApp _ (.ofApp _ (.ofBase .ofOrB) (.ofBase .ofFalseB)) (.ofBVar 0)) (.ofBVar 0))
 
 theorem LamThmValid.false_or_eq_id : LamThmValid lval [] LamTerm.false_or_eq_id := by
   intro lctx'; rw [pushLCtxs_nil]; exists LamWF.false_or_eq_id; intro _ b; rfl
@@ -1858,7 +1858,7 @@ def LamTerm.true_or_eq_true : LamTerm := .mkForallEF (.base .bool) (.mkEq (.base
   (.app (.base .bool) (.app (.base .bool) (.base .orb) (.base .trueb)) (.bvar 0)) (.base .trueb))
 
 def LamWF.true_or_eq_true : LamWF ltv ⟨lctx, LamTerm.true_or_eq_true, .base .prop⟩ :=
-  .mkForallEF (.mkEq (.ofApp _ (.ofApp _ (.ofBase .ofOrB') (.ofBase .ofTrueB')) (.ofBVar 0)) (.ofBase .ofTrueB'))
+  .mkForallEF (.mkEq (.ofApp _ (.ofApp _ (.ofBase .ofOrB) (.ofBase .ofTrueB)) (.ofBVar 0)) (.ofBase .ofTrueB))
 
 theorem LamThmValid.true_or_eq_true : LamThmValid lval [] LamTerm.true_or_eq_true := by
   intro lctx'; rw [pushLCtxs_nil]; exists LamWF.true_or_eq_true; intro _ b; rfl
@@ -1867,7 +1867,7 @@ def LamTerm.ofPropSpec : LamTerm := .mkForallEF (.base .prop) (.mkEq (.base .pro
   (.mkEq (.base .bool) (.app (.base .prop) (.base .ofProp) (.bvar 0)) (.base .trueb)) (.bvar 0))
 
 def LamWF.ofPropSpec : LamWF ltv ⟨lctx, LamTerm.ofPropSpec, .base .prop⟩ :=
-  .mkForallEF (.mkEq (.mkEq (.ofApp _ (.ofBase .ofOfProp') (.ofBVar 0)) (.ofBase .ofTrueB')) (.ofBVar 0))
+  .mkForallEF (.mkEq (.mkEq (.ofApp _ (.ofBase .ofOfProp) (.ofBVar 0)) (.ofBase .ofTrueB)) (.ofBVar 0))
 
 theorem LamThmValid.ofPropSpec : LamThmValid lval [] LamTerm.ofPropSpec := by
   intro lctx'; rw [pushLCtxs_nil]; exists LamWF.ofPropSpec; intro _ x
